SEARpred_set.sml
@@ -7,6 +7,31 @@ e0
  “!A B f:A->B. tof(Tpm(f))  = f”));
 
 
+val Tpm_tof_inv = prove_store("Tpm_tof_inv",
+e0
+(flip_tac >> rpt strip_tac >> irule is_Tpm >>
+ rw[tof_def])
+(form_goal
+ “!A B f:mem(Exp(A,B)). Tpm(tof(f))  = f”));
+
+
+val Tpm_eq_eq = prove_store("Tpm_eq_eq",
+e0
+(rpt strip_tac >> dimp_tac >> rpt strip_tac >> arw[] >> 
+ irule $ iffLR FUN_EXT >>
+ once_rw[GSYM Tpm_def] >> arw[])
+(form_goal “!A B f1:A->B f2. Tpm(f1) = Tpm(f2) <=> f1 = f2”));
+
+
+val tof_eq_eq = prove_store("tof_eq_eq",
+e0
+(rpt strip_tac >> dimp_tac >> strip_tac >> arw[] >>
+ qby_tac ‘Tpm(tof(f)) = Tpm(tof(g))’ >-- arw[]>> fs[Tpm_tof_inv] )
+(form_goal
+ “!A B f:mem(Exp(A,B)) g. tof(f)  = tof(g) <=> f = g”));
+
+
+
 val IN_Sing = prove_store("IN_Sing",
 e0
 (rw[Sing_def,Sg_def])
